generational/spec/GC.Gen.CheneyGraphReadiness.fsti
@@ -14,6 +14,7 @@ module MH = GC.Spec.MajorHeap
 module Obj = GC.Spec.Object
 module SpecHeap = GC.Spec.Heap
 module Fields = GC.Spec.Fields
+module SpecAlloc = GC.Spec.Allocator
 module SpecMajorAlloc = GC.Spec.MajorAllocator
 module PromotionDemand = GC.Gen.PromotionDemand
 module ChunkedCheney = GC.Gen.ChunkedCheney
@@ -2213,12 +2214,8 @@ val chunked_cheney_promote_after_minor_promotion_head_preflight_single_chunk_fro
     (requires
       minor_wf minor /\
       alloc_fuel > 1 /\
-      GenInv.chunked_collection_heap_shape
-        minor (MH.single_chunk_major_heap major) fp alloc_fuel /\
-      SpecMajorAlloc.major_fl_chain_terminates
-        (MH.single_chunk_major_heap major) fp alloc_fuel = true /\
-      GenInv.chunked_chain_objects_blue
-        (MH.single_chunk_major_heap major) fp alloc_fuel /\
+      alloc_fuel == SpecAlloc.alloc_search_fuel /\
+      GenInv.collection_heap_shape minor major fp /\
       RBridge.roots_valid_nonblue roots major /\
       RBridge.major_field_zero_no_minor minor major /\
       (let chunked_major = MH.single_chunk_major_heap major in
@@ -2245,12 +2242,8 @@ val chunked_cheney_collect_after_minor_promotion_head_preflight_single_chunk_fro
     (requires
       minor_wf minor /\
       alloc_fuel > 1 /\
-      GenInv.chunked_collection_heap_shape
-        minor (MH.single_chunk_major_heap major) fp alloc_fuel /\
-      SpecMajorAlloc.major_fl_chain_terminates
-        (MH.single_chunk_major_heap major) fp alloc_fuel = true /\
-      GenInv.chunked_chain_objects_blue
-        (MH.single_chunk_major_heap major) fp alloc_fuel /\
+      alloc_fuel == SpecAlloc.alloc_search_fuel /\
+      GenInv.collection_heap_shape minor major fp /\
       RBridge.roots_valid_nonblue roots major /\
       RBridge.major_field_zero_no_minor minor major /\
       (let chunked_major = MH.single_chunk_major_heap major in
@@ -2278,12 +2271,8 @@ val chunked_cheney_promote_after_minor_promotion_head_preflight_single_chunk_fro
       minor_wf minor /\
       alloc_fuel > 1 /\
       Fields.well_formed_heap major /\
-      GenInv.chunked_collection_heap_shape
-        minor (MH.single_chunk_major_heap major) fp alloc_fuel /\
-      SpecMajorAlloc.major_fl_chain_terminates
-        (MH.single_chunk_major_heap major) fp alloc_fuel = true /\
-      GenInv.chunked_chain_objects_blue
-        (MH.single_chunk_major_heap major) fp alloc_fuel /\
+      alloc_fuel == SpecAlloc.alloc_search_fuel /\
+      GenInv.collection_heap_shape minor major fp /\
       RBridge.roots_valid_nonblue roots major /\
       RBridge.major_field_zero_no_minor minor major /\
       (let chunked_major = MH.single_chunk_major_heap major in
@@ -2306,12 +2295,8 @@ val chunked_cheney_collect_after_minor_promotion_head_preflight_single_chunk_fro
       minor_wf minor /\
       alloc_fuel > 1 /\
       Fields.well_formed_heap major /\
-      GenInv.chunked_collection_heap_shape
-        minor (MH.single_chunk_major_heap major) fp alloc_fuel /\
-      SpecMajorAlloc.major_fl_chain_terminates
-        (MH.single_chunk_major_heap major) fp alloc_fuel = true /\
-      GenInv.chunked_chain_objects_blue
-        (MH.single_chunk_major_heap major) fp alloc_fuel /\
+      alloc_fuel == SpecAlloc.alloc_search_fuel /\
+      GenInv.collection_heap_shape minor major fp /\
       RBridge.roots_valid_nonblue roots major /\
       RBridge.major_field_zero_no_minor minor major /\
       (let chunked_major = MH.single_chunk_major_heap major in
@@ -2368,12 +2353,8 @@ val chunked_cheney_gc_correct_after_preflight_policy_and_post_reachable_image_si
     (requires
       minor_wf minor /\
       alloc_fuel > 1 /\
-      GenInv.chunked_collection_heap_shape
-        minor (MH.single_chunk_major_heap major) fp alloc_fuel /\
-      SpecMajorAlloc.major_fl_chain_terminates
-        (MH.single_chunk_major_heap major) fp alloc_fuel = true /\
-      GenInv.chunked_chain_objects_blue
-        (MH.single_chunk_major_heap major) fp alloc_fuel /\
+      alloc_fuel == SpecAlloc.alloc_search_fuel /\
+      GenInv.collection_heap_shape minor major fp /\
       RBridge.roots_valid_nonblue base_roots major /\
       RBridge.major_field_zero_no_minor minor major /\
       (SpecMajorAlloc.major_fl_head_wosize
@@ -2409,12 +2390,8 @@ val chunked_cheney_gc_correct_after_preflight_full_policy_and_post_reachable_ima
     (requires
       minor_wf minor /\
       alloc_fuel > 1 /\
-      GenInv.chunked_collection_heap_shape
-       minor (MH.single_chunk_major_heap major) fp alloc_fuel /\
-      SpecMajorAlloc.major_fl_chain_terminates
-       (MH.single_chunk_major_heap major) fp alloc_fuel = true /\
-      GenInv.chunked_chain_objects_blue
-       (MH.single_chunk_major_heap major) fp alloc_fuel /\
+      alloc_fuel == SpecAlloc.alloc_search_fuel /\
+      GenInv.collection_heap_shape minor major fp /\
       RBridge.roots_valid_nonblue base_roots major /\
       RBridge.major_field_zero_no_minor minor major /\
       (let chunked_major = MH.single_chunk_major_heap major in
@@ -2463,12 +2440,8 @@ val chunked_cheney_gc_correct_after_preflight_full_policy_and_post_reachable_ima
       minor_wf minor /\
       alloc_fuel > 1 /\
       Fields.well_formed_heap major /\
-      GenInv.chunked_collection_heap_shape
-       minor (MH.single_chunk_major_heap major) fp alloc_fuel /\
-      SpecMajorAlloc.major_fl_chain_terminates
-       (MH.single_chunk_major_heap major) fp alloc_fuel = true /\
-      GenInv.chunked_chain_objects_blue
-       (MH.single_chunk_major_heap major) fp alloc_fuel /\
+      alloc_fuel == SpecAlloc.alloc_search_fuel /\
+      GenInv.collection_heap_shape minor major fp /\
       RBridge.roots_valid_nonblue base_roots major /\
       RBridge.major_field_zero_no_minor minor major /\
       (let chunked_major = MH.single_chunk_major_heap major in
